Prefix: : <http://www.semanticweb.org/thoma/ontologies/2020/3/f21bd#>
Prefix: dc: <http://purl.org/dc/elements/1.1/>
Prefix: owl: <http://www.w3.org/2002/07/owl#>
Prefix: rdf: <http://www.w3.org/1999/02/22-rdf-syntax-ns#>
Prefix: rdfs: <http://www.w3.org/2000/01/rdf-schema#>
Prefix: skos: <http://www.w3.org/2004/02/skos/core#>
Prefix: xml: <http://www.w3.org/XML/1998/namespace>
Prefix: xsd: <http://www.w3.org/2001/XMLSchema#>



Ontology: <http://www.semanticweb.org/thoma/ontologies/2020/3/f21bd>


Annotations: 
    dc:contributor "Thomas Di Martino",
    dc:creator "Thomas Di Martino",
    dc:date 04.2020,
    dc:description "Movie ontology for the CourseWork nÂ°2 of F21BD - Heriot Watt"

AnnotationProperty: dc:contributor

    
AnnotationProperty: dc:creator

    
AnnotationProperty: dc:date

    
AnnotationProperty: dc:description

    
AnnotationProperty: rdfs:comment

    
AnnotationProperty: rdfs:isDefinedBy

    
AnnotationProperty: rdfs:label

    
AnnotationProperty: skos:prefLabel

    
Datatype: rdf:PlainLiteral

    
Datatype: xsd:dateTime

    
Datatype: xsd:integer

    
Datatype: xsd:nonNegativeInteger

    
Datatype: xsd:string

    
ObjectProperty: hasActedIn

    Annotations: 
        rdfs:comment "Defines the link between and actor and the movie he/she has worked in."@en
    
    SubPropertyOf: 
        hasWorkedIn
    
    Domain: 
        Actor
    
    
ObjectProperty: hasDirected

    Annotations: 
        rdfs:comment "Defines the link between a director and the movie she/he has directed"@en
    
    SubPropertyOf: 
        hasWorkedIn
    
    Domain: 
        Director
    
    
ObjectProperty: hasGenre

    Annotations: 
        rdfs:comment "Defines the link between a movie and a genre"@en
    
    Domain: 
        Movie
    
    Range: 
        Genre
    
    
ObjectProperty: hasProduced

    Annotations: 
        rdfs:comment "Defines the link between a producer and a movie he/she has produced"@en
    
    SubPropertyOf: 
        hasWorkedIn
    
    Domain: 
        Producer
    
    
ObjectProperty: hasWorkedIn

    Annotations: 
        rdfs:comment "Design a superclass of objectProperties linking MovieWorkers to movies. It adds an abstraction layers to prevent to define \"Movie\" as being the range of each objectProperty describing a \"hasWorkedIn\" action (whether it is for acting, producing, directing etc...). 

Hence, any sub property of this current property will inherit of this range, and will just have to provide the adequate domain."@en
    
    SubPropertyOf: 
        owl:topObjectProperty
    
    Domain: 
        MovieWorker
    
    Range: 
        Movie
    
    
ObjectProperty: owl:topObjectProperty

    
DataProperty: hasDuration

    Annotations: 
        rdfs:comment "Defines the duration of a movie"@en
    
    Domain: 
        Movie
    
    
DataProperty: hasImdbId

    Annotations: 
        rdfs:comment "Defines a IMDB ID of a movie. If a movie has an IMDB ID, it automatically also becomes a ImdbMovie"@en
    
    Domain: 
        Movie
    
    
DataProperty: hasReleaseYear

    Annotations: 
        rdfs:comment "Defines the release year of a movie"@en
    
    Domain: 
        Movie
    
    
DataProperty: hasTitle

    Annotations: 
        rdfs:comment "Defines the title of a movie"@en
    
    Domain: 
        Movie
    
    
DataProperty: hasTmdbId

    Annotations: 
        rdfs:comment "Defines the TMDB ID of a movie. If a movie has a TMDB ID, it automatically also becomes a TmdbMovie"@en
    
    Domain: 
        Movie
    
    
Class: <http://xmlns.com/foaf/0.1/Person>

    Annotations: 
        rdfs:isDefinedBy "foaf:"
    
    SubClassOf: 
        DomainThing
    
    
Class: ActionGenre

    Annotations: 
        rdfs:comment "Movies defined by risk and stakes, with action-oriented content"@en
    
    SubClassOf: 
        Genre
    
    
Class: Actor

    SubClassOf: 
        MovieWorker
    
    
Class: AnimationGenre

    Annotations: 
        rdfs:comment "Defined by inanimate objects being manipulated with the intention of making them appear as living things."@en
    
    SubClassOf: 
        Genre
    
    
Class: ComedyGenre

    Annotations: 
        rdfs:comment "Genre in which events and the way they are related are intended to induce laughter, disrigarding whether the story is macabre, zany, or simply amusing."@en
    
    SubClassOf: 
        Genre
    
    
Class: CrimeGenre

    Annotations: 
        rdfs:comment "Crime Genre displays interactions betwee the two sides of the criminal justice system, without focus on legislation, or civil suits."@en
    
    SubClassOf: 
        Genre
    
    
Class: Director

    SubClassOf: 
        MovieWorker
    
    
Class: DomainThing

    Annotations: 
        rdfs:label "DomainThing"@en,
        skos:prefLabel "Domain Thing"@en
    
    
Class: DramaGenre

    Annotations: 
        rdfs:comment "Drama is defined by conflict. It aims at being as realistic as possible and distances itself from the usual sensationalism from other genres. Emotions are the main focus, by relying on intense situations."@en
    
    SubClassOf: 
        Genre
    
    
Class: ExperimentalGenre

    Annotations: 
        rdfs:comment "Experimental genre usually foregoes a cohesive narrative to, intentionally, be unfit for any other particular genre."@en
    
    SubClassOf: 
        Genre
    
    
Class: FantasyGenre

    Annotations: 
        rdfs:comment "Defined by setting its actions inside a fictional universe, with unrealistic outcomes and natural laws."@en
    
    SubClassOf: 
        Genre
    
    
Class: FeatureMovie

    Annotations: 
        rdfs:comment "Any movie long enough to be considered as the main featured movie on a television evening night. Rules on considering a movie to be a feature movie may differ, we chose to consider any movie more than 40min long to be a feature movie."@en
    
    EquivalentTo: 
        Movie
         and (hasDuration some xsd:nonNegativeInteger[> "40"^^xsd:nonNegativeInteger])
    
    SubClassOf: 
        Movie
    
    DisjointWith: 
        ShortMovie
    
    
Class: Genre

    Annotations: 
        rdfs:comment "Defines the main categories of movies as classes. Specific subgenres can then be defined as individuals of these respective classes.

These classes are NOT disjoint as a movie can be a mix of multiple genres (it is the case of the majority of movies)."@en
    
    SubClassOf: 
        DomainThing
    
    
Class: HistoricalGenre

    Annotations: 
        rdfs:comment "Historical Genre regroups both historically accurate movies with biographies and memoirs as well as fictional movies placed under a relatively accuracte depiction of a historical event."@en
    
    SubClassOf: 
        Genre
    
    
Class: HorrorGenre

    Annotations: 
        rdfs:comment "Centered upon terrific or macabre events for the thrill and the heart pumping feelings that the depicted terrible events may confer."@en
    
    SubClassOf: 
        Genre
    
    
Class: Movie

    SubClassOf: 
        DomainThing,
        hasReleaseYear some xsd:dateTime,
        hasTitle some xsd:string
    
    
Class: MovieImdb

    Annotations: 
        rdfs:comment "Any movie registered as an Imdb movie (i.e. any movie entered with an imdb id)"@en
    
    EquivalentTo: 
        Movie
         and (hasImdbId some xsd:string)
    
    SubClassOf: 
        Movie,
        hasImdbId some xsd:string
    
    
Class: MovieTmdb

    Annotations: 
        rdfs:comment "Any movie registered as being a Tmdb movie (i.e. any movie with a tmdb id)"@en
    
    EquivalentTo: 
        Movie
         and (hasTmdbId some xsd:string)
    
    SubClassOf: 
        Movie,
        hasTmdbId some xsd:string
    
    
Class: MovieWorker

    Annotations: 
        rdfs:comment "Any Person working on a Movie is considered a Movie worker, from being on set to being responsible for the special effects."@en
    
    SubClassOf: 
        <http://xmlns.com/foaf/0.1/Person>
    
    
Class: OtherGenres

    Annotations: 
        rdfs:comment "Any genre that does not enter any other category"@en
    
    SubClassOf: 
        Genre
    
    
Class: Producer

    SubClassOf: 
        MovieWorker
    
    
Class: RomanceGenre

    Annotations: 
        rdfs:comment "Defined by intimate relationships with, in some cases, darker twist to illustrate the natural conflicts linked to intimacy or love."@en
    
    SubClassOf: 
        Genre
    
    
Class: ScienceFictionGenre

    Annotations: 
        rdfs:comment "Defined by a mixture of fiction and science, hence its name, the SciFi genre tries to explain the unknown using technology and science, whereas Fantasy relies on magic and mysticism."@en
    
    SubClassOf: 
        Genre
    
    
Class: ShortMovie

    Annotations: 
        rdfs:comment "Any movie not long enough to be considered as the main featured movie on a television evening night. We chose to consider any movie less than 40min long to be a short movie."@en
    
    EquivalentTo: 
        Movie
         and (hasDuration some xsd:nonNegativeInteger[< "40"^^xsd:nonNegativeInteger])
    
    SubClassOf: 
        Movie
    
    DisjointWith: 
        FeatureMovie
    
    
Class: ThrillerGenre

    Annotations: 
        rdfs:comment "Centered around the emotions, it tries to bring suspense and anxiety to the heart of the viewer."@en
    
    SubClassOf: 
        Genre
    
    
Class: User

    SubClassOf: 
        <http://xmlns.com/foaf/0.1/Person>
    
    
Class: WesternGenre

    Annotations: 
        rdfs:comment "Defined by their setting and time period, western movies can take place in the American West, from Missouri to the Pacific Ocean. Usually set in the 19th century, they can display violence or non-violence."@en
    
    SubClassOf: 
        Genre
    
    
Individual: Absurdist

    Types: 
        ExperimentalGenre
    
    
Individual: Action

    Types: 
        ActionGenre
    
    
Individual: Biography

    Types: 
        HistoricalGenre
    
    
Individual: Comedy

    Types: 
        ComedyGenre
    
    
Individual: DarkFantasy

    Types: 
        FantasyGenre
    
    
Individual: Ghost

    Types: 
        HorrorGenre
    
    
Individual: Historical_Epic

    Types: 
        HistoricalGenre
    
    
Individual: Horror

    Types: 
        HorrorGenre
    
    
Individual: Musical

    Types: 
        OtherGenres
    
    
Individual: Myth

    Types: 
        FantasyGenre
    
    
Individual: Occult

    Types: 
        HorrorGenre
    
    
Individual: PeriodRomance

    Types: 
        RomanceGenre
    
    
Individual: TestActor1

    Facts:  
     hasActedIn  TestFeatureAction
    
    
Individual: TestDirector1

    Facts:  
     hasDirected  TestMovieNoGenre
    
    
Individual: TestFeatureAction

    Facts:  
     hasGenre  Action,
     hasDuration  70,
     hasImdbId  "a1b2c3d4",
     hasReleaseYear  1995,
     hasTitle  "TestFeatureAction"
    
    
Individual: TestMovieNoGenre

    
Individual: TestShortHorrorComedy

    Facts:  
     hasGenre  Comedy,
     hasGenre  Horror,
     hasDuration  35,
     hasReleaseYear  1998,
     hasTitle  "TestShortHorrorComedy"
    
    
Individual: Western

    Types: 
        WesternGenre
    
    
Individual: WesternSpaghetti

    Types: 
        WesternGenre
    
    
